Get rid of ccExp'

Launchbury/CoCallAnalysisBinds.thy
@@ -1,14 +1,14 @@
 theory CoCallAnalysisBinds
-imports CoCallAnalysis AEnv  "AList-Utils-HOLCF"
+imports CoCallAnalysis AEnv  "AList-Utils-HOLCF" "Arity-Nominal""CoCallGraph-Nominal"
 begin
 
 context CoCallAnalysis
 begin
 definition ccBind :: "var \<Rightarrow> exp \<Rightarrow> ((AEnv \<times> CoCalls) \<rightarrow> CoCalls)"
-  where "ccBind v e = (\<Lambda> (ae, G).  if (v--v\<notin>G) \<or> \<not> isLam e then cc_restr (fv e) (ccExp' e \<cdot> (ae v)) else ccSquare (fv e))"
+  where "ccBind v e = (\<Lambda> (ae, G).  if (v--v\<notin>G) \<or> \<not> isLam e then cc_restr (fv e) (fup\<cdot>(ccExp e)\<cdot>(ae v)) else ccSquare (fv e))"
 (* paper has:  \<or> ae v = up\<cdot>0, but that is not monotone! But should give the same result. *)
 
-lemma ccBind_eq: "ccBind v e \<cdot> (ae, G) = (if (v--v\<notin>G) \<or> \<not> isLam e then cc_restr (fv e) (ccExp' e \<cdot> (ae v)) else ccSquare (fv e))"
+lemma ccBind_eq: "ccBind v e \<cdot> (ae, G) = (if (v--v\<notin>G) \<or> \<not> isLam e then cc_restr (fv e) (fup\<cdot>(ccExp e)\<cdot>(ae v)) else ccSquare (fv e))"
   unfolding ccBind_def
   apply (rule cfun_beta_Pair)
   apply (rule cont_if_else_above)
@@ -97,7 +97,7 @@ lemma ccBind_cong[fundef_cong]:
   "cccexp1 e = cccexp2 e \<Longrightarrow> CoCallAnalysis.ccBind cccexp1 x e = CoCallAnalysis.ccBind cccexp2 x e "
   apply (rule cfun_eqI)
   apply (case_tac xa)
-  apply (auto simp add: CoCallAnalysis.ccBind_eq  cong: ccExp'_cong)
+  apply (auto simp add: CoCallAnalysis.ccBind_eq)
   done
 
 lemma ccBinds_cong[fundef_cong]:
