Launchbury/CoCallAnalysis.thy
@@ -1,29 +1,9 @@
 theory CoCallAnalysis
-imports Terms "Arity-Nominal" "CoCallGraph-Nominal" Substitution
+imports Terms Arity CoCallGraph
 begin
 
 locale CoCallAnalysis =
   fixes ccExp :: "exp \<Rightarrow> Arity \<rightarrow> CoCalls"
-begin
-
-definition ccExp' :: "exp \<Rightarrow> Arity\<^sub>\<bottom> \<rightarrow> CoCalls"
-  where "ccExp' e = fup \<cdot> (ccExp e)"
-
-lemma ccExp'_simps[simp]:
-  "ccExp' e \<cdot> \<bottom> = \<bottom>"
-  "ccExp' e \<cdot> (up\<cdot>n) = ccExp e \<cdot> n"
-  unfolding ccExp'_def by simp_all
-
-end
-
-lemma ccExp'_eqvt[eqvt]:
-  "\<pi> \<bullet> (CoCallAnalysis.ccExp' ccexp e) = CoCallAnalysis.ccExp' (\<pi> \<bullet> ccexp) (\<pi> \<bullet> e)"
-  unfolding CoCallAnalysis.ccExp'_def
-  by perm_simp rule
-
-lemma ccExp'_cong: 
-  "cccexp1 e = cccexp2 e \<Longrightarrow> CoCallAnalysis.ccExp' cccexp1 e = CoCallAnalysis.ccExp' cccexp2 e"
-  unfolding CoCallAnalysis.ccExp'_def by simp
 
 locale CoCallAnalyisHeap = 
   fixes ccHeap :: "heap \<Rightarrow> exp \<Rightarrow> Arity \<rightarrow> CoCalls"
